added locally_equivalent_solved for transformation T1

lambda.v
@@ -1,7 +1,7 @@
 Require Import List ssreflect.
 Import ListNotations.
 Require Import PeanoNat.
-Require Import Nat.
+Require Import Nat Lia.
 
 
 (* equivalent to rose_tree (nat * nat) *)
@@ -638,7 +638,8 @@ Inductive solved (ap : aposition) (theta : lookup_contents) :
     | solved_const gs n x ts rs:
       get_arena_subterm TS ap = Some (tm n (x + length theta) ts) ->
       length ts = length rs ->
-      Forall2 (fun _ t => match t with tm nt _ _ => nt = 0 end) gs ts ->
+      length gs = length ts ->
+      Forall (fun t => match t with tm nt _ _ => nt = 0 end) ts ->
       (forall g j r, In (g, (j, r)) (combine gs (combine (seq 0 (length rs)) rs)) ->
         solved (extend_ap ap [j]) theta g r) ->
       solved ap theta (node (ap, theta) gs) (node x rs).
@@ -843,7 +844,7 @@ T1 is t[b/n].
 TODO: restate as an application of substitution
  *)
 
-Fixpoint trans_T1 (t:term) (p:position) (t':term) : term :=
+Definition trans_T1 (t:term) (p:position) (t':term) : term :=
   replace_subterm t' p t.
 
 
@@ -862,8 +863,117 @@ g.tr. then if we replace the subterm at p with any term, the resulting
 term is a solution.
 
  *)
-Lemma trans_T1_correct:
-  forall t args ap theta gtr res t'' p t',
+
+Fixpoint get_apositions (gtr: game_tree) : list aposition :=
+  match gtr with
+  | node (ap, _) children => ap :: flat_map get_apositions children
+  end.
+
+Inductive locally_equivalent : option term -> option term -> Prop :=
+  | locally_equivalent_Some n x ts ts' : length ts = length ts' -> locally_equivalent (Some (tm n x ts)) (Some (tm n x ts'))
+  | locally_equivalent_None : locally_equivalent None None.
+
+Lemma locally_equivalent_elim ot ot' n x args : 
+  locally_equivalent ot ot' ->
+  ot = Some (tm n x args) ->
+  exists args', length args = length args' /\ ot' = Some (tm n x args').
+Proof.
+  case=> >; last done.
+  move=> ? [*]. subst.
+  eexists. by split; last done.
+Qed.
+
+Arguments in_combine_l {A B l l' x y}.
+Arguments in_split {A x l}.
+
+Lemma get_arena_subterm_extend_ap ts ap n x rs j:
+  get_arena_subterm ts ap = Some (tm n x rs) ->
+  get_arena_subterm ts (extend_ap ap [j]) = nth_error rs j.
+Proof.
+  move: ap => [i p] /=.
+  move: (nth_error ts i)=> [t|]; last done.
+  (* TODO provable subterm property from rose_tree framework *)
+Admitted.
+
+Lemma combine_map {A B A' B' : Type} (f : A -> A') (g : B -> B') (l1 : list A) (l2 : list B) :
+  combine (map f l1) (map g l2) = map (fun ab => (f (fst ab), g (snd ab))) (combine l1 l2).
+Proof.
+  elim: l1 l2; first done.
+  move=> a l1 IH [|b l2]; first done.
+  by rewrite /= IH.
+Qed.
+
+Lemma locally_equivalent_solved ts ts' ap theta gtr res:
+  solved ts ap theta gtr res ->
+  Forall (fun ap' => locally_equivalent (get_arena_subterm ts ap') (get_arena_subterm ts' ap')) (get_apositions gtr) ->
+  solved ts' ap theta gtr res.
+Proof.
+  move=> H. elim: H ts'.
+  - move=> {}ap {}theta n x args nap theta' {}gtr r.
+    move=> /locally_equivalent_elim Hap Hx Hgtr IH ts' /=.
+    move=> /Forall_cons_iff [/Hap [?] [H'args H'ap]] /Forall_app [/IH] + _.
+    rewrite H'args. by apply: solved_var; eassumption.
+  - move=> {}ap {}theta gs n x {}rs' rs.
+    move=> /[dup] H''ap /locally_equivalent_elim Hap Hlen H'len Hrs' IH' IH ts' /=.
+    move=> /Forall_cons_iff [/Hap [rs''] [H'rs'' H'ap]] Hgs.
+    apply: solved_const.
+    + eassumption.
+    + by rewrite -H'rs''.
+    + by rewrite -H'rs''.
+    + (* the game will continue in subtrees, which are also locally equivalent *)
+      have Hrs'': forall g j r,
+        In (g, (j, r)) (combine gs (combine (seq 0 (length rs')) rs)) ->
+        locally_equivalent (nth_error rs' j) (nth_error rs'' j).
+      { move=> g j r. rewrite !Hlen.
+        move: H''ap => /get_arena_subterm_extend_ap <-.
+        move: H'ap => /get_arena_subterm_extend_ap <-.
+        move=> /[dup] Hgjr /IH' {}IH'.
+        move: Hgs => /Forall_forall. apply.
+        move: (extend_ap ap [j]) IH' => ? IH'.
+        move: Hgjr=> /in_combine_l /in_split [?] [?] ?. subst gs.
+        rewrite flat_map_app /=.
+        apply: in_or_app. right. apply: in_or_app. left.
+        by case: IH'=> * /=; left. }
+      move: Hrs' Hlen H'len H'rs'' Hrs''. clear=> Hrs'.
+      elim: Hrs' rs'' gs rs; first by case.
+      move=> [???] ? -> _ IH'' [|[???] ?]; first done.
+      move=> [|? gs]; first done.
+      move=> [|? rs]; first done.
+      move=> /= [/IH'' {}IH''] [/IH'' {}IH''] [/IH'' {}IH''] Hequiv. constructor.
+      * move: (Hequiv _ 0 _ (or_introl eq_refl)) => /= H.
+        by inversion H.
+      * apply: IH'' => ? j ? H. apply: (Hequiv _ (S j) _). right.
+        rewrite -seq_shift -(map_id rs) -(map_id gs) !combine_map.
+        apply /in_map_iff. eexists. by split; last by eassumption.
+    + move=> g j r Hgjr. apply: IH; first done.
+      move: Hgjr => /in_combine_l /in_split [?] [?] ?. subst gs.
+      rewrite flat_map_app in Hgs.
+      by move: Hgs => /Forall_app [?] /= /Forall_app [].
+Qed.
+
+Arguments node {A}.
+
+Fixpoint rose_tree_size {A : Type} (tr : rose_tree A) : nat :=
+  match tr with
+  | node _ ts => 1 + list_sum (map rose_tree_size ts)
+  end.
+
+(* induction principle on rose trees *)
+Lemma rose_tree_ind' {A : Type} (P : rose_tree A -> Prop) :
+  (forall (v : A) (l : list (rose_tree A)), Forall P l -> P (node v l)) ->
+  forall tr, P tr.
+Proof.
+  move=> H. elim /(Nat.measure_induction _ (@rose_tree_size A)).
+  move=> [v children] IH. apply: H.
+  elim: children IH.
+  - by constructor.
+  - move=> ?? IH IH'. constructor.
+    + apply: IH'=> /=. lia.
+    + apply: IH => /= *. apply: IH'=> /=. lia.
+Qed.
+
+(* application of locally_equivalent_solved *)
+Lemma trans_T1_correct t args ap theta gtr res t'' p t':
   solved (t :: args) ap theta gtr res ->
   fold_tree (check_occurrence p) gtr = false -> (* p does not occur in gtr *)
   t'' = trans_T1 t p t' ->
@@ -872,20 +982,21 @@ Lemma trans_T1_correct:
   TTT t t'' -> *)
   solved (t'' :: args) ap theta gtr res.
 Proof.
-  intros t args ap theta gtr res t'' p t'.
-  intro.
-  inversion H.
-  * (* solved_var *)
-    intros.
-    eapply solved_var.
-    ** (* solved_var in assumption *)
-      admit.
-    ** (* solved_const in assumption *)
-      admit.
-  * (* solved_const *)
-    intros.
+  move=> /locally_equivalent_solved + Hp ->. apply.
+  have: Forall (fun ap' => ap' <> (0, p)) (get_apositions gtr).
+  { (* should be easy *) admit. }
+  apply: Forall_impl=> - [[|?] p'].
+  - move=> ? /=. have ?: p' <> p by congruence.
+    rewrite /trans_T1.
+    (* this does not hold because one needs that p is not a prefix of p'
+       will require that if a position occurs in a game tree, then all prefixes occur in the game tree
+       is this true for arbitrary theta? *)
     admit.
-Admitted.                  
+  - move=> /= _. case: (nth_error args _); last by constructor.
+    move=> ?. case: (subterm _ p'); last by constructor.
+    move=> [???]. by constructor.
+Admitted.
+             
 
 Lemma test_trans_T1_ex1_0: trans_T1 ex1_0 [] 0 = Some ex1_2.
 Proof.
